Alloy/C/Shim.lean
@@ -9,31 +9,136 @@ open Lean
 
 namespace Alloy.C
 
-/-- A single command in a C Shim. -/
-structure ShimCmd where
-  /-- The Lean syntax of the command. -/
-  stx : Cmd
-  /-- Start of the command in the **C** source. -/
-  startPos : String.Pos
-  /-- End of the command in the **C** source. -/
-  endPose : String.Pos
-  deriving Inhabited
+/--
+A piece of shim `Syntax` that has been reprinted via `reprintShim` and thus its
+nodes are tagged with synthetic `SourceInfo` detailing its span within the shim.
+-/
+abbrev ShimSyntax := Syntax
+
+/-- Converts all non-whitespace characters of the string to whitespace. -/
+def toWhitespace (str : String) : String :=
+  str.map fun c => if c.isWhitespace then c else ' '
+
+/-- `Lean.Syntax.reprintLeaf`, but transforms comments into whitespace. -/
+def reprintLeaf (val : String) : SourceInfo → String
+| .original lead _ trail _ =>
+  s!"{toWhitespace lead.toString}{val}{toWhitespace trail.toString}"
+| _  => s!" {val} "
 
 /--
-Find the C source position within the command
-corresponding to the `leanPos` in the Lean source.
+Like `Lean.Syntax.reprint`, but transforms comments into whitespace and
+tags nodes with `SourceInfo` noting their position in the reprinted code.
 -/
-def ShimCmd.findPos? (self : ShimCmd) (leanPos : String.Pos) : Option String.Pos := do
-  let some headPos := self.stx.raw.getPos? | failure
-  let some tailPos := self.stx.raw.getTailPos? | failure
-  if headPos < leanPos && leanPos < tailPos then
-    return leanPos - headPos + self.startPos
-  else
+partial def reprint (stx : Syntax) (startPos : String.Pos := 0) : Option (String × ShimSyntax) := do
+  match stx with
+  | .atom info val =>
+    return (reprintLeaf val info, stx)
+  | .ident info rawVal _ _ =>
+    return (reprintLeaf rawVal.toString info, stx)
+  | .node _ kind args =>
+    let mut s := ""
+    let mut args' := #[]
+    if kind = choiceKind then
+      let (s0, arg0) ← reprint (← args[0]?) startPos
+      args' := args'.push arg0
+      for arg in args[1:] do
+        let (s', arg') ← reprint arg startPos
+        args' := args'.push arg'
+        guard (s0 == s')
+      s := s ++ s0
+    else
+      for arg in args do
+        let pos := startPos + s.endPos
+        let (s', arg') ← reprint arg pos
+        args' := args'.push arg'
+        s := s ++ s'
+    return (s, Syntax.node (.synthetic startPos (startPos + s.endPos)) kind args')
+  | _ => failure
+
+/-- Computes the `bsize` of the reprinted `Syntax` in the shim source. -/
+def ShimSyntax.bsize : ShimSyntax → Nat
+| .atom info val => sizeLeaf val.toSubstring info
+| .ident info rawVal .. => sizeLeaf rawVal info
+| .node (.synthetic head tail) _ _ => tail.byteIdx - head.byteIdx
+| _ => 0
+where
+  sizeLeaf (val : Substring) : SourceInfo → Nat
+  | .original lead _ trail _ => lead.bsize + val.bsize + trail.bsize
+  | _  => val.bsize + 2
+
+/--
+Find the position within the `ShimSyntax`
+corresponding to the `leanPos` in the Lean source.
+
+The algorithm Traverses the syntax tree top-to-bottom, left-to-right to find
+a leaf whose range includes `leanPos`. It assumes nothing about the relationship
+between Lean source information of elements within the tree. Thus, it is very
+linear in its performance.
+-/
+partial def ShimSyntax.leanPosToShim? (stx : ShimSyntax)
+(leanPos : String.Pos) (shimStartPos : String.Pos := 0) : Option String.Pos := do
+  if let .node info _ args := stx then
+    --
+    let .synthetic shimStartPos _ := info | failure
+    let mut startPos := shimStartPos
+    for arg in args do
+      if let some pos := leanPosToShim? arg leanPos startPos then
+        return pos
+      startPos := startPos + ⟨ShimSyntax.bsize arg⟩
     failure
+  else
+    let some leanHeadPos := stx.getPos? | failure
+    let some leanTailPos := stx.getTailPos? | failure
+    if leanHeadPos ≤ leanPos && leanPos < leanTailPos then
+      return leanPos - leanHeadPos + shimStartPos
+    failure
+
+/-- Computes the start and end of the `atom`/`ident` in the Lean source. -/
+def ShimSyntax.leafRange? : ShimSyntax → Option (String.Pos × String.Pos)
+| .atom (.original _ head _ tail) .. => (head, tail)
+| .atom (.synthetic head tail) .. => (head, tail)
+| .ident (.original _ head _ tail) .. => (head, tail)
+| .ident (.synthetic head tail) .. => (head, tail)
+| _ => none
+
+/--
+Find the Lean position within the
+`ShimSyntax` corresponding to `shimPos` in the shim.
+
+This algorithms assumes the shim `SourceInfo` position of nodes are
+monotonically increasing from left-to-right and lower node's range is a subset
+of a higher node's range in the syntax tree. In other words, it assumes the
+syntax has not been re-ordered since it was tagged with source information
+(e.g., via `reprint`).
+-/
+partial def ShimSyntax.shimPosToLean? (stx : ShimSyntax)
+(shimPos : String.Pos) (shimHeadPos shimTailPos : String.Pos := 0) : Option String.Pos := do
+  if let .node info _ args := stx then
+    let .synthetic shimHeadPos shimTailPos := info | failure
+    if shimHeadPos ≠ shimTailPos then -- e.g., null nodes
+      if shimHeadPos > shimPos then failure
+      if shimTailPos ≤ shimPos then failure
+    let mut headPos := shimHeadPos
+    for arg in args do
+      let tailPos := headPos + ⟨ShimSyntax.bsize arg⟩
+      if let some pos := shimPosToLean? arg shimPos headPos tailPos then
+        return pos
+      headPos := tailPos
+  else
+    let (leanHeadPos, leanTailPos) ← stx.leafRange?
+    if shimHeadPos ≤ shimPos && shimPos < shimTailPos then
+      let shimOff := shimPos - shimHeadPos
+      let leanLen := leanTailPos - leanHeadPos
+      let leanPos := leanHeadPos + min shimOff leanLen
+      return leanPos
+  failure
+
+/-- A single, reprinted command in a C shim. -/
+abbrev ShimCmd := Cmd
 
 /-- A C shim -- an array of commands with shim source position information. -/
 structure Shim where
-  cmds : Array ShimCmd
+  cmds : Array ShimSyntax
   text : FileMap
   deriving Inhabited
 
@@ -57,9 +162,9 @@ Add a command to the shim.
 Fails if the command could not be reprinted.
 -/
 def pushCmd? (cmd : Cmd) (self : Shim) : Option Shim := do
-  let startPos := self.text.source.endPos
-  let code := self.text.source ++ (← cmd.raw.reprint).trim ++ "\n"
-  return ⟨self.cmds.push ⟨cmd, startPos, code.endPos⟩, FileMap.ofString code⟩
+  let (code, cmd) ← reprint cmd.raw self.text.source.endPos
+  let code := self.text.source ++ code ++ "\n"
+  return ⟨self.cmds.push cmd, FileMap.ofString code⟩
 
 /--
 Appends an `Array` of commands to the shim.
@@ -69,10 +174,10 @@ def appendCmds? (cmds : Array Cmd) (self : Shim) : Except Cmd Shim := do
   let mut shimCmds := self.cmds
   let mut code := self.text.source
   for cmd in cmds do
-    let startPos := code.endPos
-    let some cmdCode := cmd.raw.reprint | throw cmd
-    code := code ++ cmdCode.trim ++ "\n"
-    shimCmds := shimCmds.push ⟨cmd, startPos, code.endPos⟩
+    let some (cmdCode, cmd) := reprint cmd.raw code.endPos
+      | throw cmd
+    code := code ++ cmdCode ++ "\n"
+    shimCmds := shimCmds.push cmd
   return ⟨shimCmds, FileMap.ofString code⟩
 
 /--
@@ -83,8 +188,15 @@ def ofCmds (cmds : Array Cmd) : Shim :=
   Shim.empty.appendCmds? cmds |>.toOption.getD Shim.empty
 
 /--
-Find the C source position within the shim
+Find the position within the C shim
 corresponding to the `leanPos` in the Lean source.
 -/
-def findPos? (self : Shim) (leanPos : String.Pos) : Option String.Pos :=
-  self.cmds.findSome? (·.findPos? leanPos)
+def leanPosToC? (self : Shim) (leanPos : String.Pos) : Option String.Pos :=
+  self.cmds.findSome? (·.leanPosToShim? leanPos)
+
+/--
+Find the position within the shim's Lean syntax
+corresponding to the `cPos` in the C shim.
+-/
+def cPosToLean? (self : Shim) (cPos : String.Pos) : Option String.Pos :=
+  self.cmds.findSome? (·.shimPosToLean? cPos)
