Alloy/Util/Server.lean
@@ -15,21 +15,3 @@ def nullUri : DocumentUri :=
     "file:///nul"
   else
     "file:///dev/null"
-
-/-- Like `chainLspRequestHandler` but without the `IO.initializing` check. -/
-def forceChainLspRequestHandler (method : String)
-    paramType [FromJson paramType]
-    respType [FromJson respType] [ToJson respType]
-    (handler : paramType → RequestTask respType → RequestM (RequestTask respType)) : IO Unit := do
-  if let some oldHandler ← lookupLspRequestHandler method then
-    let handle := fun j => do
-      let t ← oldHandler.handle j
-      let t := t.map fun x => x.bind fun j => FromJson.fromJson? j |>.mapError fun e =>
-        IO.userError s!"Failed to parse original LSP response for `{method}` when chaining: {e}"
-      let params ← liftExcept <| parseRequestParams paramType j
-      let t ← handler params t
-      pure <| t.map <| Except.map ToJson.toJson
-
-    requestHandlers.modify fun rhs => rhs.insert method {oldHandler with handle}
-  else
-    throw <| IO.userError s!"Failed to chain LSP request handler for '{method}': no initial handler registered"
