Alloy/Util/Server/Worker.lean
@@ -3,6 +3,7 @@ Copyright (c) 2022 Mac Malone. All rights reserved.
 Released under Apache 2.0 license as described in the file LICENSE.
 Authors: Mac Malone
 -/
+import Lean.Server.AsyncList
 import Lean.Data.Lsp.Communication
 import Alloy.Util.Server.Initialize
 
@@ -19,12 +20,51 @@ abbrev RequestMap (α) := Std.RBMap RequestID α compare
 /- State for an `LsWorker`. -/
 structure LsState where
   nextID : Nat := 0
+  messages : IO.AsyncList IO.Error Message := .nil
   pendingResponses : RequestMap Json := {}
+
+namespace LsState
+
+def saveResponse (id : RequestID) (result : Json) (self : LsState) : LsState :=
+  {self with pendingResponses := self.pendingResponses.insert id result}
+
+-- TODO: Handle non-response messages
+partial def waitResponse (expectedID : RequestID)
+: ExceptT IO.Error (StateM LsState) (Option Json) := do
+  match (← get).messages with
+  | .nil => return .none
+  | .cons m ms =>
+    modify ({· with messages := ms})
+    if let .response id result := m then
+      if id == expectedID then
+        return result
+      else
+        modify (·.saveResponse id result)
+    waitResponse expectedID
+  | .delayed ms =>
+    modify ({· with messages := ← ms.get})
+    waitResponse expectedID
+
+def takePendingResponse? (id : RequestID) : StateM LsState <| Option Json := fun self => do
+  if let some result := self.pendingResponses.find? id then
+    (.some result, {self with pendingResponses := self.pendingResponses.erase id})
+  else
+    (.none, self)
+
+def getOrWaitResponse (expectedID : RequestID)
+: ExceptT IO.Error (StateM LsState) (Option Json) := do
+  if let some result ← takePendingResponse? expectedID then
+    return result
+  waitResponse expectedID
+
+end LsState
 
 /-- A running language server process -/
 structure LsWorker where
   child : IO.Process.Child ipcStdioConfig
   state : IO.Ref LsState
+  capabilities : ServerCapabilities := {}
+  info? : Option ServerInfo := none
 
 namespace LsWorker
 
@@ -41,7 +81,7 @@ def withTextDocument [Monad m] [MonadLiftT IO m] [MonadFinally m]
 (self : LsWorker) (uri : DocumentUri) (text : String) (languageId : String)
 (act : m α) (version := 0) : m α := do
   let dop : DidOpenTextDocumentParams := ⟨{uri, version, text, languageId}⟩
-  self.notify "textDocument/didOpen"  dop
+  self.notify "textDocument/didOpen" dop
   try
     act
   finally
@@ -63,29 +103,44 @@ def takePendingResponse? (self : LsWorker) (id : RequestID) : BaseIO (Option Jso
     | some result => (some result, {s with pendingResponses := rs.erase id})
     | none => (none, s)
 
--- TODO: Use separate task to read messages and handle non-response messages
-partial def readUntilResponse (self : LsWorker) (expectedID : RequestID) : IO Json := do
-  if let some result ← self.takePendingResponse? expectedID then
-    return result
-  let msg ← self.stdout.readLspMessage
-  if let .response id result := msg then
-    if id == expectedID then
-      return result
-    else
-      self.state.modify fun s => {s with pendingResponses := s.pendingResponses.insert id result}
-  self.readUntilResponse expectedID
+def readUntilResponse (self : LsWorker) (expectedID : RequestID) : IO Json := do
+  match (← self.state.modifyGet <| LsState.getOrWaitResponse expectedID) with
+  | .ok (some result) => return result
+  | .ok none => throw <| IO.userError <|
+    s!"Language server quit without responding to request `{expectedID}`"
+  | .error e => throw e
 
 def readUntilResponseAs (self : LsWorker) (expectedID : RequestID) (α) [FromJson α] : IO α := do
   let result ← self.readUntilResponse expectedID
   match fromJson? result with
   | .ok v => pure v
   | .error inner => throw <| IO.userError <|
-    s!"Unexpected result '{result.compress}'\n{inner}"
+    s!"Unexpected result for request `{expectedID}`:\n'{result.compress}'\n{inner}"
+
+def call [ToJson α] [FromJson β] (self : LsWorker) (method : String) (param : α) : IO β := do
+  let id ← self.request method param
+  self.readUntilResponseAs id β
+
+/-- Auxiliary function for `readMessagesAsync` -/
+partial def readMessagesAsyncAux (self : LsWorker)
+: BaseIO (Task <| Except IO.Error <| IO.AsyncList IO.Error Message) := IO.asTask do
+  let msg ← self.stdout.readLspMessage
+  let nextTask ← self.readMessagesAsyncAux
+  return .cons msg <| .delayed nextTask
+
+/-- Asynchronously read all messages from the language server and build a lazy list of them. -/
+def readMessagesAsync (self : LsWorker) : BaseIO (IO.AsyncList IO.Error Message) :=
+  .delayed <$> self.readMessagesAsyncAux
 
 def init (cmd : String) (args : Array String := #[]) (params : InitializeParams) : IO LsWorker := do
   let child ← IO.Process.spawn {cmd, args, toStdioConfig := ipcStdioConfig}
   let ls : LsWorker := {child, state := ← IO.mkRef {}}
-  let id ← ls.request "initialize" params
-  let ⟨_, _⟩ ← ls.stdout.readLspResponseAs id Json
+  let messages ← ls.readMessagesAsync
+  ls.state.modify ({· with messages})
+  let (⟨capabilities, info?⟩ : InitializeResult) ← ls.call "initialize" params
   ls.notify "initialized" InitializedParams.mk
-  return ls
+  return {ls with capabilities, info?}
+
+def exit (self : LsWorker) : IO PUnit := do
+  let (_ : Json) ← self.call "shutdown" Json.null
+  self.notify "exit" Json.null
